curve25519-dalek/translated/FunsExternal.lean
@@ -27,12 +27,16 @@ axiom core.array.from_fn
   core.ops.function.FnMut F Std.Usize T) :
   F → Result (Array T N)
 
-/-- [core::borrow::{impl core::borrow::Borrow<T> for T}::borrow]:
-    Source: '/rustc/library/core/src/borrow.rs', lines 214:4-214:26
-    Name pattern: [core::borrow::{core::borrow::Borrow<@T, @T>}::borrow]
+/-- [core::array::{impl core::iter::traits::collect::IntoIterator<&'a mut T, core::slice::iter::IterMut<'a, T>> for &'a mut [T; N]}::into_iter]:
+    Source: '/rustc/library/core/src/array/mod.rs', lines 376:4-376:40
+    Name pattern: [core::array::{core::iter::traits::collect::IntoIterator<&'a mut [@T; @N], &'a mut @T, core::slice::iter::IterMut<'a, @T>>}::into_iter]
     Visibility: public -/
-@[rust_fun "core::borrow::{core::borrow::Borrow<@T, @T>}::borrow"]
-axiom core.borrow.Borrow.Blanket.borrow {T : Type} : T → Result T
+@[rust_fun
+  "core::array::{core::iter::traits::collect::IntoIterator<&'a mut [@T; @N], &'a mut @T, core::slice::iter::IterMut<'a, @T>>}::into_iter"]
+axiom MutAArray.Insts.CoreIterTraitsCollectIntoIteratorMutATIterMut.into_iter
+  {T : Type} {N : Std.Usize} :
+  Array T N → Result ((core.slice.iter.IterMut T) × (core.slice.iter.IterMut
+    T → Array T N))
 
 /-- [core::fmt::{impl core::fmt::Debug for str}::fmt]:
     Source: '/rustc/library/core/src/fmt/mod.rs', lines 2932:4-2932:50
@@ -199,26 +203,41 @@ axiom core.slice.iter.IterMut.Insts.ZeroizeZeroize.zeroize
   core.slice.iter.IterMut Z → Result ((core.slice.iter.IterMut Z) ×
     (core.slice.iter.IterMut Z → core.slice.iter.IterMut Z))
 
-/-- [curve25519_dalek::backend::serial::scalar_mul::pippenger::{impl curve25519_dalek::traits::VartimeMultiscalarMul<curve25519_dalek::edwards::EdwardsPoint> for curve25519_dalek::backend::serial::scalar_mul::pippenger::Pippenger}::optional_multiscalar_mul]:
+/-- [curve25519_dalek::backend::serial::scalar_mul::pippenger::{impl curve25519_dalek::traits::VartimeMultiscalarMul<curve25519_dalek::edwards::EdwardsPoint::x86_64-unknown-linux-gnu> for curve25519_dalek::backend::serial::scalar_mul::pippenger::Pippenger}::optional_multiscalar_mul]:
     Source: 'curve25519-dalek/src/backend/serial/scalar_mul/pippenger.rs', lines 67:4-176:5
     Visibility: public -/
 axiom
-  backend.serial.scalar_mul.pippenger.Pippenger.Insts.Curve25519_dalekTraitsVartimeMultiscalarMulEdwardsPoint.optional_multiscalar_mul
+  backend.serial.scalar_mul.pippenger.Pippenger.Insts.«Curve25519_dalekTraitsVartimeMultiscalarMulEdwardsPointx86_64-unknown-linux-gnu».optional_multiscalar_mul
   {I : Type} {J : Type} {Clause0_Item : Type} {Clause0_IntoIter : Type}
   {Clause2_IntoIter : Type} (coreitertraitscollectIntoIteratorInst :
   core.iter.traits.collect.IntoIterator I Clause0_Item Clause0_IntoIter)
   (coreborrowBorrowClause0_ItemScalarInst : core.borrow.Borrow Clause0_Item
   scalar.Scalar)
-  (coreitertraitscollectIntoIteratorJOptionEdwardsPointClause2_IntoIterInst :
-  core.iter.traits.collect.IntoIterator J (Option edwards.EdwardsPoint)
-  Clause2_IntoIter) :
-  I → J → Result (Option edwards.EdwardsPoint)
+  («coreitertraitscollectIntoIteratorJOptionEdwardsPointx86_64-unknown-linux-gnuClause2_IntoIterInst»
+  : core.iter.traits.collect.IntoIterator J (Option
+  edwards.EdwardsPoint.«x86_64-unknown-linux-gnu») Clause2_IntoIter) :
+  I → J → Result (Option edwards.EdwardsPoint.«x86_64-unknown-linux-gnu»)
 
-/-- [curve25519_dalek::backend::serial::scalar_mul::precomputed_straus::{impl curve25519_dalek::traits::VartimePrecomputedMultiscalarMul<curve25519_dalek::edwards::EdwardsPoint> for curve25519_dalek::backend::serial::scalar_mul::precomputed_straus::VartimePrecomputedStraus}::optional_mixed_multiscalar_mul]:
+/-- [curve25519_dalek::backend::serial::scalar_mul::pippenger::{impl curve25519_dalek::traits::VartimeMultiscalarMul<curve25519_dalek::edwards::EdwardsPoint::i686-unknown-linux-gnu> for curve25519_dalek::backend::serial::scalar_mul::pippenger::Pippenger}::optional_multiscalar_mul]:
+    Source: 'curve25519-dalek/src/backend/serial/scalar_mul/pippenger.rs', lines 67:4-176:5
+    Visibility: public -/
+axiom
+  backend.serial.scalar_mul.pippenger.Pippenger.Insts.«Curve25519_dalekTraitsVartimeMultiscalarMulEdwardsPointi686-unknown-linux-gnu».optional_multiscalar_mul
+  {I : Type} {J : Type} {Clause0_Item : Type} {Clause0_IntoIter : Type}
+  {Clause2_IntoIter : Type} (coreitertraitscollectIntoIteratorInst :
+  core.iter.traits.collect.IntoIterator I Clause0_Item Clause0_IntoIter)
+  (coreborrowBorrowClause0_ItemScalarInst : core.borrow.Borrow Clause0_Item
+  scalar.Scalar)
+  («coreitertraitscollectIntoIteratorJOptionEdwardsPointi686-unknown-linux-gnuClause2_IntoIterInst»
+  : core.iter.traits.collect.IntoIterator J (Option
+  edwards.EdwardsPoint.«i686-unknown-linux-gnu») Clause2_IntoIter) :
+  I → J → Result (Option edwards.EdwardsPoint.«i686-unknown-linux-gnu»)
+
+/-- [curve25519_dalek::backend::serial::scalar_mul::precomputed_straus::{impl curve25519_dalek::traits::VartimePrecomputedMultiscalarMul<curve25519_dalek::edwards::EdwardsPoint::x86_64-unknown-linux-gnu> for curve25519_dalek::backend::serial::scalar_mul::precomputed_straus::VartimePrecomputedStraus::x86_64-unknown-linux-gnu}::optional_mixed_multiscalar_mul]:
     Source: 'curve25519-dalek/src/backend/serial/scalar_mul/precomputed_straus.rs', lines 57:4-127:5
     Visibility: public -/
 axiom
-  backend.serial.scalar_mul.precomputed_straus.VartimePrecomputedStraus.Insts.Curve25519_dalekTraitsVartimePrecomputedMultiscalarMulEdwardsPoint.optional_mixed_multiscalar_mul
+  backend.serial.scalar_mul.precomputed_straus.VartimePrecomputedStraus.«x86_64-unknown-linux-gnu».Insts.«Curve25519_dalekTraitsVartimePrecomputedMultiscalarMulEdwardsPointx86_64-unknown-linux-gnu».optional_mixed_multiscalar_mul
   {I : Type} {J : Type} {K : Type} {Clause0_Item : Type} {Clause0_IntoIter :
   Type} {Clause2_Item : Type} {Clause2_IntoIter : Type} {Clause4_IntoIter :
   Type} (coreitertraitscollectIntoIteratorInst :
@@ -228,30 +247,67 @@ axiom
   core.iter.traits.collect.IntoIterator J Clause2_Item Clause2_IntoIter)
   (coreborrowBorrowClause2_ItemScalarInst : core.borrow.Borrow Clause2_Item
   scalar.Scalar)
-  (coreitertraitscollectIntoIteratorKOptionEdwardsPointClause4_IntoIterInst :
-  core.iter.traits.collect.IntoIterator K (Option edwards.EdwardsPoint)
-  Clause4_IntoIter) :
-  backend.serial.scalar_mul.precomputed_straus.VartimePrecomputedStraus → I
-    → J → K → Result (Option edwards.EdwardsPoint)
+  («coreitertraitscollectIntoIteratorKOptionEdwardsPointx86_64-unknown-linux-gnuClause4_IntoIterInst»
+  : core.iter.traits.collect.IntoIterator K (Option
+  edwards.EdwardsPoint.«x86_64-unknown-linux-gnu») Clause4_IntoIter) :
+  backend.serial.scalar_mul.precomputed_straus.VartimePrecomputedStraus.«x86_64-unknown-linux-gnu»
+    → I → J → K → Result (Option
+    edwards.EdwardsPoint.«x86_64-unknown-linux-gnu»)
 
-/-- [curve25519_dalek::backend::serial::scalar_mul::precomputed_straus::{impl curve25519_dalek::traits::VartimePrecomputedMultiscalarMul<curve25519_dalek::edwards::EdwardsPoint> for curve25519_dalek::backend::serial::scalar_mul::precomputed_straus::VartimePrecomputedStraus}::new]:
+/-- [curve25519_dalek::backend::serial::scalar_mul::precomputed_straus::{impl curve25519_dalek::traits::VartimePrecomputedMultiscalarMul<curve25519_dalek::edwards::EdwardsPoint::x86_64-unknown-linux-gnu> for curve25519_dalek::backend::serial::scalar_mul::precomputed_straus::VartimePrecomputedStraus::x86_64-unknown-linux-gnu}::new]:
     Source: 'curve25519-dalek/src/backend/serial/scalar_mul/precomputed_straus.rs', lines 36:4-47:5
     Visibility: public -/
 axiom
-  backend.serial.scalar_mul.precomputed_straus.VartimePrecomputedStraus.Insts.Curve25519_dalekTraitsVartimePrecomputedMultiscalarMulEdwardsPoint.new
+  backend.serial.scalar_mul.precomputed_straus.VartimePrecomputedStraus.«x86_64-unknown-linux-gnu».Insts.«Curve25519_dalekTraitsVartimePrecomputedMultiscalarMulEdwardsPointx86_64-unknown-linux-gnu».new
   {I : Type} {Clause0_Item : Type} {Clause0_IntoIter : Type}
   (coreitertraitscollectIntoIteratorInst :
   core.iter.traits.collect.IntoIterator I Clause0_Item Clause0_IntoIter)
-  (coreborrowBorrowClause0_ItemEdwardsPointInst : core.borrow.Borrow
-  Clause0_Item edwards.EdwardsPoint) :
+  («coreborrowBorrowClause0_ItemEdwardsPointx86_64-unknown-linux-gnuInst» :
+  core.borrow.Borrow Clause0_Item
+  edwards.EdwardsPoint.«x86_64-unknown-linux-gnu») :
   I → Result
-    backend.serial.scalar_mul.precomputed_straus.VartimePrecomputedStraus
+    backend.serial.scalar_mul.precomputed_straus.VartimePrecomputedStraus.«x86_64-unknown-linux-gnu»
 
-/-- [curve25519_dalek::backend::serial::scalar_mul::straus::{impl curve25519_dalek::traits::MultiscalarMul<curve25519_dalek::edwards::EdwardsPoint> for curve25519_dalek::backend::serial::scalar_mul::straus::Straus}::multiscalar_mul]:
+/-- [curve25519_dalek::backend::serial::scalar_mul::precomputed_straus::{impl curve25519_dalek::traits::VartimePrecomputedMultiscalarMul<curve25519_dalek::edwards::EdwardsPoint::i686-unknown-linux-gnu> for curve25519_dalek::backend::serial::scalar_mul::precomputed_straus::VartimePrecomputedStraus::i686-unknown-linux-gnu}::optional_mixed_multiscalar_mul]:
+    Source: 'curve25519-dalek/src/backend/serial/scalar_mul/precomputed_straus.rs', lines 57:4-127:5
+    Visibility: public -/
+axiom
+  backend.serial.scalar_mul.precomputed_straus.VartimePrecomputedStraus.«i686-unknown-linux-gnu».Insts.«Curve25519_dalekTraitsVartimePrecomputedMultiscalarMulEdwardsPointi686-unknown-linux-gnu».optional_mixed_multiscalar_mul
+  {I : Type} {J : Type} {K : Type} {Clause0_Item : Type} {Clause0_IntoIter :
+  Type} {Clause2_Item : Type} {Clause2_IntoIter : Type} {Clause4_IntoIter :
+  Type} (coreitertraitscollectIntoIteratorInst :
+  core.iter.traits.collect.IntoIterator I Clause0_Item Clause0_IntoIter)
+  (coreborrowBorrowClause0_ItemScalarInst : core.borrow.Borrow Clause0_Item
+  scalar.Scalar) (coreitertraitscollectIntoIteratorInst1 :
+  core.iter.traits.collect.IntoIterator J Clause2_Item Clause2_IntoIter)
+  (coreborrowBorrowClause2_ItemScalarInst : core.borrow.Borrow Clause2_Item
+  scalar.Scalar)
+  («coreitertraitscollectIntoIteratorKOptionEdwardsPointi686-unknown-linux-gnuClause4_IntoIterInst»
+  : core.iter.traits.collect.IntoIterator K (Option
+  edwards.EdwardsPoint.«i686-unknown-linux-gnu») Clause4_IntoIter) :
+  backend.serial.scalar_mul.precomputed_straus.VartimePrecomputedStraus.«i686-unknown-linux-gnu»
+    → I → J → K → Result (Option
+    edwards.EdwardsPoint.«i686-unknown-linux-gnu»)
+
+/-- [curve25519_dalek::backend::serial::scalar_mul::precomputed_straus::{impl curve25519_dalek::traits::VartimePrecomputedMultiscalarMul<curve25519_dalek::edwards::EdwardsPoint::i686-unknown-linux-gnu> for curve25519_dalek::backend::serial::scalar_mul::precomputed_straus::VartimePrecomputedStraus::i686-unknown-linux-gnu}::new]:
+    Source: 'curve25519-dalek/src/backend/serial/scalar_mul/precomputed_straus.rs', lines 36:4-47:5
+    Visibility: public -/
+axiom
+  backend.serial.scalar_mul.precomputed_straus.VartimePrecomputedStraus.«i686-unknown-linux-gnu».Insts.«Curve25519_dalekTraitsVartimePrecomputedMultiscalarMulEdwardsPointi686-unknown-linux-gnu».new
+  {I : Type} {Clause0_Item : Type} {Clause0_IntoIter : Type}
+  (coreitertraitscollectIntoIteratorInst :
+  core.iter.traits.collect.IntoIterator I Clause0_Item Clause0_IntoIter)
+  («coreborrowBorrowClause0_ItemEdwardsPointi686-unknown-linux-gnuInst» :
+  core.borrow.Borrow Clause0_Item
+  edwards.EdwardsPoint.«i686-unknown-linux-gnu») :
+  I → Result
+    backend.serial.scalar_mul.precomputed_straus.VartimePrecomputedStraus.«i686-unknown-linux-gnu»
+
+/-- [curve25519_dalek::backend::serial::scalar_mul::straus::{impl curve25519_dalek::traits::MultiscalarMul<curve25519_dalek::edwards::EdwardsPoint::x86_64-unknown-linux-gnu> for curve25519_dalek::backend::serial::scalar_mul::straus::Straus}::multiscalar_mul]:
     Source: 'curve25519-dalek/src/backend/serial/scalar_mul/straus.rs', lines 103:4-144:5
     Visibility: public -/
 axiom
-  backend.serial.scalar_mul.straus.Straus.Insts.Curve25519_dalekTraitsMultiscalarMulEdwardsPoint.multiscalar_mul
+  backend.serial.scalar_mul.straus.Straus.Insts.«Curve25519_dalekTraitsMultiscalarMulEdwardsPointx86_64-unknown-linux-gnu».multiscalar_mul
   {I : Type} {J : Type} {Clause0_Item : Type} {Clause0_IntoIter : Type}
   {Clause2_Item : Type} {Clause2_IntoIter : Type}
   (coreitertraitscollectIntoIteratorInst :
@@ -259,44 +315,92 @@ axiom
   (coreborrowBorrowClause0_ItemScalarInst : core.borrow.Borrow Clause0_Item
   scalar.Scalar) (coreitertraitscollectIntoIteratorInst1 :
   core.iter.traits.collect.IntoIterator J Clause2_Item Clause2_IntoIter)
-  (coreborrowBorrowClause2_ItemEdwardsPointInst : core.borrow.Borrow
-  Clause2_Item edwards.EdwardsPoint) :
-  I → J → Result edwards.EdwardsPoint
+  («coreborrowBorrowClause2_ItemEdwardsPointx86_64-unknown-linux-gnuInst» :
+  core.borrow.Borrow Clause2_Item
+  edwards.EdwardsPoint.«x86_64-unknown-linux-gnu») :
+  I → J → Result edwards.EdwardsPoint.«x86_64-unknown-linux-gnu»
 
-/-- [curve25519_dalek::backend::serial::scalar_mul::straus::{impl curve25519_dalek::traits::VartimeMultiscalarMul<curve25519_dalek::edwards::EdwardsPoint> for curve25519_dalek::backend::serial::scalar_mul::straus::Straus}::optional_multiscalar_mul]:
+/-- [curve25519_dalek::backend::serial::scalar_mul::straus::{impl curve25519_dalek::traits::MultiscalarMul<curve25519_dalek::edwards::EdwardsPoint::i686-unknown-linux-gnu> for curve25519_dalek::backend::serial::scalar_mul::straus::Straus}::multiscalar_mul]:
+    Source: 'curve25519-dalek/src/backend/serial/scalar_mul/straus.rs', lines 103:4-144:5
+    Visibility: public -/
+axiom
+  backend.serial.scalar_mul.straus.Straus.Insts.«Curve25519_dalekTraitsMultiscalarMulEdwardsPointi686-unknown-linux-gnu».multiscalar_mul
+  {I : Type} {J : Type} {Clause0_Item : Type} {Clause0_IntoIter : Type}
+  {Clause2_Item : Type} {Clause2_IntoIter : Type}
+  (coreitertraitscollectIntoIteratorInst :
+  core.iter.traits.collect.IntoIterator I Clause0_Item Clause0_IntoIter)
+  (coreborrowBorrowClause0_ItemScalarInst : core.borrow.Borrow Clause0_Item
+  scalar.Scalar) (coreitertraitscollectIntoIteratorInst1 :
+  core.iter.traits.collect.IntoIterator J Clause2_Item Clause2_IntoIter)
+  («coreborrowBorrowClause2_ItemEdwardsPointi686-unknown-linux-gnuInst» :
+  core.borrow.Borrow Clause2_Item
+  edwards.EdwardsPoint.«i686-unknown-linux-gnu») :
+  I → J → Result edwards.EdwardsPoint.«i686-unknown-linux-gnu»
+
+/-- [curve25519_dalek::backend::serial::scalar_mul::straus::{impl curve25519_dalek::traits::VartimeMultiscalarMul<curve25519_dalek::edwards::EdwardsPoint::x86_64-unknown-linux-gnu> for curve25519_dalek::backend::serial::scalar_mul::straus::Straus}::optional_multiscalar_mul]:
     Source: 'curve25519-dalek/src/backend/serial/scalar_mul/straus.rs', lines 159:4-200:5
     Visibility: public -/
 axiom
-  backend.serial.scalar_mul.straus.Straus.Insts.Curve25519_dalekTraitsVartimeMultiscalarMulEdwardsPoint.optional_multiscalar_mul
+  backend.serial.scalar_mul.straus.Straus.Insts.«Curve25519_dalekTraitsVartimeMultiscalarMulEdwardsPointx86_64-unknown-linux-gnu».optional_multiscalar_mul
   {I : Type} {J : Type} {Clause0_Item : Type} {Clause0_IntoIter : Type}
   {Clause2_IntoIter : Type} (coreitertraitscollectIntoIteratorInst :
   core.iter.traits.collect.IntoIterator I Clause0_Item Clause0_IntoIter)
   (coreborrowBorrowClause0_ItemScalarInst : core.borrow.Borrow Clause0_Item
   scalar.Scalar)
-  (coreitertraitscollectIntoIteratorJOptionEdwardsPointClause2_IntoIterInst :
-  core.iter.traits.collect.IntoIterator J (Option edwards.EdwardsPoint)
-  Clause2_IntoIter) :
-  I → J → Result (Option edwards.EdwardsPoint)
+  («coreitertraitscollectIntoIteratorJOptionEdwardsPointx86_64-unknown-linux-gnuClause2_IntoIterInst»
+  : core.iter.traits.collect.IntoIterator J (Option
+  edwards.EdwardsPoint.«x86_64-unknown-linux-gnu») Clause2_IntoIter) :
+  I → J → Result (Option edwards.EdwardsPoint.«x86_64-unknown-linux-gnu»)
+
+/-- [curve25519_dalek::backend::serial::scalar_mul::straus::{impl curve25519_dalek::traits::VartimeMultiscalarMul<curve25519_dalek::edwards::EdwardsPoint::i686-unknown-linux-gnu> for curve25519_dalek::backend::serial::scalar_mul::straus::Straus}::optional_multiscalar_mul]:
+    Source: 'curve25519-dalek/src/backend/serial/scalar_mul/straus.rs', lines 159:4-200:5
+    Visibility: public -/
+axiom
+  backend.serial.scalar_mul.straus.Straus.Insts.«Curve25519_dalekTraitsVartimeMultiscalarMulEdwardsPointi686-unknown-linux-gnu».optional_multiscalar_mul
+  {I : Type} {J : Type} {Clause0_Item : Type} {Clause0_IntoIter : Type}
+  {Clause2_IntoIter : Type} (coreitertraitscollectIntoIteratorInst :
+  core.iter.traits.collect.IntoIterator I Clause0_Item Clause0_IntoIter)
+  (coreborrowBorrowClause0_ItemScalarInst : core.borrow.Borrow Clause0_Item
+  scalar.Scalar)
+  («coreitertraitscollectIntoIteratorJOptionEdwardsPointi686-unknown-linux-gnuClause2_IntoIterInst»
+  : core.iter.traits.collect.IntoIterator J (Option
+  edwards.EdwardsPoint.«i686-unknown-linux-gnu») Clause2_IntoIter) :
+  I → J → Result (Option edwards.EdwardsPoint.«i686-unknown-linux-gnu»)
 
 /-- [curve25519_dalek::scalar::read_le_u64_into]:
     Source: 'curve25519-dalek/src/scalar.rs', lines 1383:0-1397:1 -/
 axiom scalar.read_le_u64_into
   : Slice Std.U8 → Slice Std.U64 → Result (Slice Std.U64)
 
-/-- [curve25519_dalek::edwards::{impl core::iter::traits::accum::Sum<T> for curve25519_dalek::edwards::EdwardsPoint}::sum]:
+/-- [curve25519_dalek::edwards::{impl core::iter::traits::accum::Sum<T> for curve25519_dalek::edwards::EdwardsPoint::x86_64-unknown-linux-gnu}::sum]:
     Source: 'curve25519-dalek/src/edwards.rs', lines 865:4-870:5
     Visibility: public -/
-axiom edwards.EdwardsPoint.Insts.CoreIterTraitsAccumSum.sum
-  {T : Type} {I : Type} (coreborrowBorrowTEdwardsPointInst : core.borrow.Borrow
-  T edwards.EdwardsPoint) (coreitertraitsiteratorIteratorInst :
-  core.iter.traits.iterator.Iterator I T) :
-  I → Result edwards.EdwardsPoint
+axiom
+  edwards.EdwardsPoint.«x86_64-unknown-linux-gnu».Insts.CoreIterTraitsAccumSum.sum
+  {T : Type} {I : Type}
+  («coreborrowBorrowTEdwardsPointx86_64-unknown-linux-gnuInst» :
+  core.borrow.Borrow T edwards.EdwardsPoint.«x86_64-unknown-linux-gnu»)
+  (coreitertraitsiteratorIteratorInst : core.iter.traits.iterator.Iterator I T)
+  :
+  I → Result edwards.EdwardsPoint.«x86_64-unknown-linux-gnu»
 
-/-- [curve25519_dalek::edwards::{impl curve25519_dalek::traits::MultiscalarMul<curve25519_dalek::edwards::EdwardsPoint> for curve25519_dalek::edwards::EdwardsPoint}::multiscalar_mul]:
+/-- [curve25519_dalek::edwards::{impl core::iter::traits::accum::Sum<T> for curve25519_dalek::edwards::EdwardsPoint::i686-unknown-linux-gnu}::sum]:
+    Source: 'curve25519-dalek/src/edwards.rs', lines 865:4-870:5
+    Visibility: public -/
+axiom
+  edwards.EdwardsPoint.«i686-unknown-linux-gnu».Insts.CoreIterTraitsAccumSum.sum
+  {T : Type} {I : Type}
+  («coreborrowBorrowTEdwardsPointi686-unknown-linux-gnuInst» :
+  core.borrow.Borrow T edwards.EdwardsPoint.«i686-unknown-linux-gnu»)
+  (coreitertraitsiteratorIteratorInst : core.iter.traits.iterator.Iterator I T)
+  :
+  I → Result edwards.EdwardsPoint.«i686-unknown-linux-gnu»
+
+/-- [curve25519_dalek::edwards::{impl curve25519_dalek::traits::MultiscalarMul<curve25519_dalek::edwards::EdwardsPoint::x86_64-unknown-linux-gnu> for curve25519_dalek::edwards::EdwardsPoint::x86_64-unknown-linux-gnu}::multiscalar_mul]:
     Source: 'curve25519-dalek/src/edwards.rs', lines 994:4-1019:5
     Visibility: public -/
 axiom
-  edwards.EdwardsPoint.Insts.Curve25519_dalekTraitsMultiscalarMulEdwardsPoint.multiscalar_mul
+  edwards.EdwardsPoint.«x86_64-unknown-linux-gnu».Insts.«Curve25519_dalekTraitsMultiscalarMulEdwardsPointx86_64-unknown-linux-gnu».multiscalar_mul
   {I : Type} {J : Type} {Clause0_Item : Type} {Clause0_IntoIter : Type}
   {Clause2_Item : Type} {Clause2_IntoIter : Type}
   (coreitertraitscollectIntoIteratorInst :
@@ -304,30 +408,63 @@ axiom
   (coreborrowBorrowClause0_ItemScalarInst : core.borrow.Borrow Clause0_Item
   scalar.Scalar) (coreitertraitscollectIntoIteratorInst1 :
   core.iter.traits.collect.IntoIterator J Clause2_Item Clause2_IntoIter)
-  (coreborrowBorrowClause2_ItemEdwardsPointInst : core.borrow.Borrow
-  Clause2_Item edwards.EdwardsPoint) :
-  I → J → Result edwards.EdwardsPoint
+  («coreborrowBorrowClause2_ItemEdwardsPointx86_64-unknown-linux-gnuInst» :
+  core.borrow.Borrow Clause2_Item
+  edwards.EdwardsPoint.«x86_64-unknown-linux-gnu») :
+  I → J → Result edwards.EdwardsPoint.«x86_64-unknown-linux-gnu»
 
-/-- [curve25519_dalek::edwards::{impl curve25519_dalek::traits::VartimeMultiscalarMul<curve25519_dalek::edwards::EdwardsPoint> for curve25519_dalek::edwards::EdwardsPoint}::optional_multiscalar_mul]:
+/-- [curve25519_dalek::edwards::{impl curve25519_dalek::traits::MultiscalarMul<curve25519_dalek::edwards::EdwardsPoint::i686-unknown-linux-gnu> for curve25519_dalek::edwards::EdwardsPoint::i686-unknown-linux-gnu}::multiscalar_mul]:
+    Source: 'curve25519-dalek/src/edwards.rs', lines 994:4-1019:5
+    Visibility: public -/
+axiom
+  edwards.EdwardsPoint.«i686-unknown-linux-gnu».Insts.«Curve25519_dalekTraitsMultiscalarMulEdwardsPointi686-unknown-linux-gnu».multiscalar_mul
+  {I : Type} {J : Type} {Clause0_Item : Type} {Clause0_IntoIter : Type}
+  {Clause2_Item : Type} {Clause2_IntoIter : Type}
+  (coreitertraitscollectIntoIteratorInst :
+  core.iter.traits.collect.IntoIterator I Clause0_Item Clause0_IntoIter)
+  (coreborrowBorrowClause0_ItemScalarInst : core.borrow.Borrow Clause0_Item
+  scalar.Scalar) (coreitertraitscollectIntoIteratorInst1 :
+  core.iter.traits.collect.IntoIterator J Clause2_Item Clause2_IntoIter)
+  («coreborrowBorrowClause2_ItemEdwardsPointi686-unknown-linux-gnuInst» :
+  core.borrow.Borrow Clause2_Item
+  edwards.EdwardsPoint.«i686-unknown-linux-gnu») :
+  I → J → Result edwards.EdwardsPoint.«i686-unknown-linux-gnu»
+
+/-- [curve25519_dalek::edwards::{impl curve25519_dalek::traits::VartimeMultiscalarMul<curve25519_dalek::edwards::EdwardsPoint::x86_64-unknown-linux-gnu> for curve25519_dalek::edwards::EdwardsPoint::x86_64-unknown-linux-gnu}::optional_multiscalar_mul]:
     Source: 'curve25519-dalek/src/edwards.rs', lines 1026:4-1054:5
     Visibility: public -/
 axiom
-  edwards.EdwardsPoint.Insts.Curve25519_dalekTraitsVartimeMultiscalarMulEdwardsPoint.optional_multiscalar_mul
+  edwards.EdwardsPoint.«x86_64-unknown-linux-gnu».Insts.«Curve25519_dalekTraitsVartimeMultiscalarMulEdwardsPointx86_64-unknown-linux-gnu».optional_multiscalar_mul
   {I : Type} {J : Type} {Clause0_Item : Type} {Clause0_IntoIter : Type}
   {Clause2_IntoIter : Type} (coreitertraitscollectIntoIteratorInst :
   core.iter.traits.collect.IntoIterator I Clause0_Item Clause0_IntoIter)
   (coreborrowBorrowClause0_ItemScalarInst : core.borrow.Borrow Clause0_Item
   scalar.Scalar)
-  (coreitertraitscollectIntoIteratorJOptionEdwardsPointClause2_IntoIterInst :
-  core.iter.traits.collect.IntoIterator J (Option edwards.EdwardsPoint)
-  Clause2_IntoIter) :
-  I → J → Result (Option edwards.EdwardsPoint)
+  («coreitertraitscollectIntoIteratorJOptionEdwardsPointx86_64-unknown-linux-gnuClause2_IntoIterInst»
+  : core.iter.traits.collect.IntoIterator J (Option
+  edwards.EdwardsPoint.«x86_64-unknown-linux-gnu») Clause2_IntoIter) :
+  I → J → Result (Option edwards.EdwardsPoint.«x86_64-unknown-linux-gnu»)
 
-/-- [curve25519_dalek::edwards::{impl curve25519_dalek::traits::VartimePrecomputedMultiscalarMul<curve25519_dalek::edwards::EdwardsPoint> for curve25519_dalek::edwards::VartimeEdwardsPrecomputation}::optional_mixed_multiscalar_mul]:
+/-- [curve25519_dalek::edwards::{impl curve25519_dalek::traits::VartimeMultiscalarMul<curve25519_dalek::edwards::EdwardsPoint::i686-unknown-linux-gnu> for curve25519_dalek::edwards::EdwardsPoint::i686-unknown-linux-gnu}::optional_multiscalar_mul]:
+    Source: 'curve25519-dalek/src/edwards.rs', lines 1026:4-1054:5
+    Visibility: public -/
+axiom
+  edwards.EdwardsPoint.«i686-unknown-linux-gnu».Insts.«Curve25519_dalekTraitsVartimeMultiscalarMulEdwardsPointi686-unknown-linux-gnu».optional_multiscalar_mul
+  {I : Type} {J : Type} {Clause0_Item : Type} {Clause0_IntoIter : Type}
+  {Clause2_IntoIter : Type} (coreitertraitscollectIntoIteratorInst :
+  core.iter.traits.collect.IntoIterator I Clause0_Item Clause0_IntoIter)
+  (coreborrowBorrowClause0_ItemScalarInst : core.borrow.Borrow Clause0_Item
+  scalar.Scalar)
+  («coreitertraitscollectIntoIteratorJOptionEdwardsPointi686-unknown-linux-gnuClause2_IntoIterInst»
+  : core.iter.traits.collect.IntoIterator J (Option
+  edwards.EdwardsPoint.«i686-unknown-linux-gnu») Clause2_IntoIter) :
+  I → J → Result (Option edwards.EdwardsPoint.«i686-unknown-linux-gnu»)
+
+/-- [curve25519_dalek::edwards::{impl curve25519_dalek::traits::VartimePrecomputedMultiscalarMul<curve25519_dalek::edwards::EdwardsPoint::x86_64-unknown-linux-gnu> for curve25519_dalek::edwards::VartimeEdwardsPrecomputation::x86_64-unknown-linux-gnu}::optional_mixed_multiscalar_mul]:
     Source: 'curve25519-dalek/src/edwards.rs', lines 1084:4-1099:5
     Visibility: public -/
 axiom
-  edwards.VartimeEdwardsPrecomputation.Insts.Curve25519_dalekTraitsVartimePrecomputedMultiscalarMulEdwardsPoint.optional_mixed_multiscalar_mul
+  edwards.VartimeEdwardsPrecomputation.«x86_64-unknown-linux-gnu».Insts.«Curve25519_dalekTraitsVartimePrecomputedMultiscalarMulEdwardsPointx86_64-unknown-linux-gnu».optional_mixed_multiscalar_mul
   {I : Type} {J : Type} {K : Type} {Clause0_Item : Type} {Clause0_IntoIter :
   Type} {Clause2_Item : Type} {Clause2_IntoIter : Type} {Clause4_IntoIter :
   Type} (coreitertraitscollectIntoIteratorInst :
@@ -337,23 +474,58 @@ axiom
   core.iter.traits.collect.IntoIterator J Clause2_Item Clause2_IntoIter)
   (coreborrowBorrowClause2_ItemScalarInst : core.borrow.Borrow Clause2_Item
   scalar.Scalar)
-  (coreitertraitscollectIntoIteratorKOptionEdwardsPointClause4_IntoIterInst :
-  core.iter.traits.collect.IntoIterator K (Option edwards.EdwardsPoint)
-  Clause4_IntoIter) :
-  edwards.VartimeEdwardsPrecomputation → I → J → K → Result (Option
-    edwards.EdwardsPoint)
+  («coreitertraitscollectIntoIteratorKOptionEdwardsPointx86_64-unknown-linux-gnuClause4_IntoIterInst»
+  : core.iter.traits.collect.IntoIterator K (Option
+  edwards.EdwardsPoint.«x86_64-unknown-linux-gnu») Clause4_IntoIter) :
+  edwards.VartimeEdwardsPrecomputation.«x86_64-unknown-linux-gnu» → I → J
+    → K → Result (Option edwards.EdwardsPoint.«x86_64-unknown-linux-gnu»)
 
-/-- [curve25519_dalek::edwards::{impl curve25519_dalek::traits::VartimePrecomputedMultiscalarMul<curve25519_dalek::edwards::EdwardsPoint> for curve25519_dalek::edwards::VartimeEdwardsPrecomputation}::new]:
+/-- [curve25519_dalek::edwards::{impl curve25519_dalek::traits::VartimePrecomputedMultiscalarMul<curve25519_dalek::edwards::EdwardsPoint::x86_64-unknown-linux-gnu> for curve25519_dalek::edwards::VartimeEdwardsPrecomputation::x86_64-unknown-linux-gnu}::new]:
     Source: 'curve25519-dalek/src/edwards.rs', lines 1068:4-1074:5
     Visibility: public -/
 axiom
-  edwards.VartimeEdwardsPrecomputation.Insts.Curve25519_dalekTraitsVartimePrecomputedMultiscalarMulEdwardsPoint.new
+  edwards.VartimeEdwardsPrecomputation.«x86_64-unknown-linux-gnu».Insts.«Curve25519_dalekTraitsVartimePrecomputedMultiscalarMulEdwardsPointx86_64-unknown-linux-gnu».new
   {I : Type} {Clause0_Item : Type} {Clause0_IntoIter : Type}
   (coreitertraitscollectIntoIteratorInst :
   core.iter.traits.collect.IntoIterator I Clause0_Item Clause0_IntoIter)
-  (coreborrowBorrowClause0_ItemEdwardsPointInst : core.borrow.Borrow
-  Clause0_Item edwards.EdwardsPoint) :
-  I → Result edwards.VartimeEdwardsPrecomputation
+  («coreborrowBorrowClause0_ItemEdwardsPointx86_64-unknown-linux-gnuInst» :
+  core.borrow.Borrow Clause0_Item
+  edwards.EdwardsPoint.«x86_64-unknown-linux-gnu») :
+  I → Result
+    edwards.VartimeEdwardsPrecomputation.«x86_64-unknown-linux-gnu»
+
+/-- [curve25519_dalek::edwards::{impl curve25519_dalek::traits::VartimePrecomputedMultiscalarMul<curve25519_dalek::edwards::EdwardsPoint::i686-unknown-linux-gnu> for curve25519_dalek::edwards::VartimeEdwardsPrecomputation::i686-unknown-linux-gnu}::optional_mixed_multiscalar_mul]:
+    Source: 'curve25519-dalek/src/edwards.rs', lines 1084:4-1099:5
+    Visibility: public -/
+axiom
+  edwards.VartimeEdwardsPrecomputation.«i686-unknown-linux-gnu».Insts.«Curve25519_dalekTraitsVartimePrecomputedMultiscalarMulEdwardsPointi686-unknown-linux-gnu».optional_mixed_multiscalar_mul
+  {I : Type} {J : Type} {K : Type} {Clause0_Item : Type} {Clause0_IntoIter :
+  Type} {Clause2_Item : Type} {Clause2_IntoIter : Type} {Clause4_IntoIter :
+  Type} (coreitertraitscollectIntoIteratorInst :
+  core.iter.traits.collect.IntoIterator I Clause0_Item Clause0_IntoIter)
+  (coreborrowBorrowClause0_ItemScalarInst : core.borrow.Borrow Clause0_Item
+  scalar.Scalar) (coreitertraitscollectIntoIteratorInst1 :
+  core.iter.traits.collect.IntoIterator J Clause2_Item Clause2_IntoIter)
+  (coreborrowBorrowClause2_ItemScalarInst : core.borrow.Borrow Clause2_Item
+  scalar.Scalar)
+  («coreitertraitscollectIntoIteratorKOptionEdwardsPointi686-unknown-linux-gnuClause4_IntoIterInst»
+  : core.iter.traits.collect.IntoIterator K (Option
+  edwards.EdwardsPoint.«i686-unknown-linux-gnu») Clause4_IntoIter) :
+  edwards.VartimeEdwardsPrecomputation.«i686-unknown-linux-gnu» → I → J
+    → K → Result (Option edwards.EdwardsPoint.«i686-unknown-linux-gnu»)
+
+/-- [curve25519_dalek::edwards::{impl curve25519_dalek::traits::VartimePrecomputedMultiscalarMul<curve25519_dalek::edwards::EdwardsPoint::i686-unknown-linux-gnu> for curve25519_dalek::edwards::VartimeEdwardsPrecomputation::i686-unknown-linux-gnu}::new]:
+    Source: 'curve25519-dalek/src/edwards.rs', lines 1068:4-1074:5
+    Visibility: public -/
+axiom
+  edwards.VartimeEdwardsPrecomputation.«i686-unknown-linux-gnu».Insts.«Curve25519_dalekTraitsVartimePrecomputedMultiscalarMulEdwardsPointi686-unknown-linux-gnu».new
+  {I : Type} {Clause0_Item : Type} {Clause0_IntoIter : Type}
+  (coreitertraitscollectIntoIteratorInst :
+  core.iter.traits.collect.IntoIterator I Clause0_Item Clause0_IntoIter)
+  («coreborrowBorrowClause0_ItemEdwardsPointi686-unknown-linux-gnuInst» :
+  core.borrow.Borrow Clause0_Item
+  edwards.EdwardsPoint.«i686-unknown-linux-gnu») :
+  I → Result edwards.VartimeEdwardsPrecomputation.«i686-unknown-linux-gnu»
 
 /-- [curve25519_dalek::montgomery::{impl core::ops::arith::Mul<&'b curve25519_dalek::scalar::Scalar, curve25519_dalek::montgomery::MontgomeryPoint> for curve25519_dalek::montgomery::MontgomeryPoint}::mul]:
     Source: 'curve25519-dalek/src/macros.rs', lines 93:12-95:13
@@ -423,31 +595,57 @@ axiom
   scalar.Scalar → montgomery.MontgomeryPoint → Result
     montgomery.MontgomeryPoint
 
-/-- [curve25519_dalek::ristretto::{curve25519_dalek::ristretto::RistrettoPoint}::double_and_compress_batch]:
+/-- [curve25519_dalek::ristretto::{curve25519_dalek::ristretto::RistrettoPoint::x86_64-unknown-linux-gnu}::double_and_compress_batch]:
     Source: 'curve25519-dalek/src/ristretto.rs', lines 566:4-663:5
     Visibility: public -/
-axiom ristretto.RistrettoPoint.double_and_compress_batch
+axiom
+  ristretto.«RistrettoPointx86_64-unknown-linux-gnu».double_and_compress_batch
   {I : Type} {Clause0_IntoIter : Type}
-  (coreitertraitscollectIntoIteratorISharedARistrettoPointClause0_IntoIterInst
-  : core.iter.traits.collect.IntoIterator I ristretto.RistrettoPoint
-  Clause0_IntoIter) :
+  («coreitertraitscollectIntoIteratorISharedARistrettoPointx86_64-unknown-linux-gnuClause0_IntoIterInst»
+  : core.iter.traits.collect.IntoIterator I
+  ristretto.RistrettoPoint.«x86_64-unknown-linux-gnu» Clause0_IntoIter) :
   I → Result (alloc.vec.Vec ristretto.CompressedRistretto)
 
-/-- [curve25519_dalek::ristretto::{impl core::iter::traits::accum::Sum<T> for curve25519_dalek::ristretto::RistrettoPoint}::sum]:
+/-- [curve25519_dalek::ristretto::{curve25519_dalek::ristretto::RistrettoPoint::i686-unknown-linux-gnu}::double_and_compress_batch]:
+    Source: 'curve25519-dalek/src/ristretto.rs', lines 566:4-663:5
+    Visibility: public -/
+axiom
+  ristretto.«RistrettoPointi686-unknown-linux-gnu».double_and_compress_batch
+  {I : Type} {Clause0_IntoIter : Type}
+  («coreitertraitscollectIntoIteratorISharedARistrettoPointi686-unknown-linux-gnuClause0_IntoIterInst»
+  : core.iter.traits.collect.IntoIterator I
+  ristretto.RistrettoPoint.«i686-unknown-linux-gnu» Clause0_IntoIter) :
+  I → Result (alloc.vec.Vec ristretto.CompressedRistretto)
+
+/-- [curve25519_dalek::ristretto::{impl core::iter::traits::accum::Sum<T> for curve25519_dalek::ristretto::RistrettoPoint::x86_64-unknown-linux-gnu}::sum]:
     Source: 'curve25519-dalek/src/ristretto.rs', lines 902:4-907:5
     Visibility: public -/
-axiom ristretto.RistrettoPoint.Insts.CoreIterTraitsAccumSum.sum
-  {T : Type} {I : Type} (coreborrowBorrowTRistrettoPointInst :
-  core.borrow.Borrow T ristretto.RistrettoPoint)
+axiom
+  ristretto.RistrettoPoint.«x86_64-unknown-linux-gnu».Insts.CoreIterTraitsAccumSum.sum
+  {T : Type} {I : Type}
+  («coreborrowBorrowTRistrettoPointx86_64-unknown-linux-gnuInst» :
+  core.borrow.Borrow T ristretto.RistrettoPoint.«x86_64-unknown-linux-gnu»)
   (coreitertraitsiteratorIteratorInst : core.iter.traits.iterator.Iterator I T)
   :
-  I → Result ristretto.RistrettoPoint
+  I → Result ristretto.RistrettoPoint.«x86_64-unknown-linux-gnu»
 
-/-- [curve25519_dalek::ristretto::{impl curve25519_dalek::traits::MultiscalarMul<curve25519_dalek::ristretto::RistrettoPoint> for curve25519_dalek::ristretto::RistrettoPoint}::multiscalar_mul]:
+/-- [curve25519_dalek::ristretto::{impl core::iter::traits::accum::Sum<T> for curve25519_dalek::ristretto::RistrettoPoint::i686-unknown-linux-gnu}::sum]:
+    Source: 'curve25519-dalek/src/ristretto.rs', lines 902:4-907:5
+    Visibility: public -/
+axiom
+  ristretto.RistrettoPoint.«i686-unknown-linux-gnu».Insts.CoreIterTraitsAccumSum.sum
+  {T : Type} {I : Type}
+  («coreborrowBorrowTRistrettoPointi686-unknown-linux-gnuInst» :
+  core.borrow.Borrow T ristretto.RistrettoPoint.«i686-unknown-linux-gnu»)
+  (coreitertraitsiteratorIteratorInst : core.iter.traits.iterator.Iterator I T)
+  :
+  I → Result ristretto.RistrettoPoint.«i686-unknown-linux-gnu»
+
+/-- [curve25519_dalek::ristretto::{impl curve25519_dalek::traits::MultiscalarMul<curve25519_dalek::ristretto::RistrettoPoint::x86_64-unknown-linux-gnu> for curve25519_dalek::ristretto::RistrettoPoint::x86_64-unknown-linux-gnu}::multiscalar_mul]:
     Source: 'curve25519-dalek/src/ristretto.rs', lines 984:4-993:5
     Visibility: public -/
 axiom
-  ristretto.RistrettoPoint.Insts.Curve25519_dalekTraitsMultiscalarMulRistrettoPoint.multiscalar_mul
+  ristretto.RistrettoPoint.«x86_64-unknown-linux-gnu».Insts.«Curve25519_dalekTraitsMultiscalarMulRistrettoPointx86_64-unknown-linux-gnu».multiscalar_mul
   {I : Type} {J : Type} {Clause0_Item : Type} {Clause0_IntoIter : Type}
   {Clause2_Item : Type} {Clause2_IntoIter : Type}
   (coreitertraitscollectIntoIteratorInst :
@@ -455,30 +653,65 @@ axiom
   (coreborrowBorrowClause0_ItemScalarInst : core.borrow.Borrow Clause0_Item
   scalar.Scalar) (coreitertraitscollectIntoIteratorInst1 :
   core.iter.traits.collect.IntoIterator J Clause2_Item Clause2_IntoIter)
-  (coreborrowBorrowClause2_ItemRistrettoPointInst : core.borrow.Borrow
-  Clause2_Item ristretto.RistrettoPoint) :
-  I → J → Result ristretto.RistrettoPoint
+  («coreborrowBorrowClause2_ItemRistrettoPointx86_64-unknown-linux-gnuInst» :
+  core.borrow.Borrow Clause2_Item
+  ristretto.RistrettoPoint.«x86_64-unknown-linux-gnu») :
+  I → J → Result ristretto.RistrettoPoint.«x86_64-unknown-linux-gnu»
 
-/-- [curve25519_dalek::ristretto::{impl curve25519_dalek::traits::VartimeMultiscalarMul<curve25519_dalek::ristretto::RistrettoPoint> for curve25519_dalek::ristretto::RistrettoPoint}::optional_multiscalar_mul]:
+/-- [curve25519_dalek::ristretto::{impl curve25519_dalek::traits::MultiscalarMul<curve25519_dalek::ristretto::RistrettoPoint::i686-unknown-linux-gnu> for curve25519_dalek::ristretto::RistrettoPoint::i686-unknown-linux-gnu}::multiscalar_mul]:
+    Source: 'curve25519-dalek/src/ristretto.rs', lines 984:4-993:5
+    Visibility: public -/
+axiom
+  ristretto.RistrettoPoint.«i686-unknown-linux-gnu».Insts.«Curve25519_dalekTraitsMultiscalarMulRistrettoPointi686-unknown-linux-gnu».multiscalar_mul
+  {I : Type} {J : Type} {Clause0_Item : Type} {Clause0_IntoIter : Type}
+  {Clause2_Item : Type} {Clause2_IntoIter : Type}
+  (coreitertraitscollectIntoIteratorInst :
+  core.iter.traits.collect.IntoIterator I Clause0_Item Clause0_IntoIter)
+  (coreborrowBorrowClause0_ItemScalarInst : core.borrow.Borrow Clause0_Item
+  scalar.Scalar) (coreitertraitscollectIntoIteratorInst1 :
+  core.iter.traits.collect.IntoIterator J Clause2_Item Clause2_IntoIter)
+  («coreborrowBorrowClause2_ItemRistrettoPointi686-unknown-linux-gnuInst» :
+  core.borrow.Borrow Clause2_Item
+  ristretto.RistrettoPoint.«i686-unknown-linux-gnu») :
+  I → J → Result ristretto.RistrettoPoint.«i686-unknown-linux-gnu»
+
+/-- [curve25519_dalek::ristretto::{impl curve25519_dalek::traits::VartimeMultiscalarMul<curve25519_dalek::ristretto::RistrettoPoint::x86_64-unknown-linux-gnu> for curve25519_dalek::ristretto::RistrettoPoint::x86_64-unknown-linux-gnu}::optional_multiscalar_mul]:
     Source: 'curve25519-dalek/src/ristretto.rs', lines 1000:4-1012:5
     Visibility: public -/
 axiom
-  ristretto.RistrettoPoint.Insts.Curve25519_dalekTraitsVartimeMultiscalarMulRistrettoPoint.optional_multiscalar_mul
+  ristretto.RistrettoPoint.«x86_64-unknown-linux-gnu».Insts.«Curve25519_dalekTraitsVartimeMultiscalarMulRistrettoPointx86_64-unknown-linux-gnu».optional_multiscalar_mul
   {I : Type} {J : Type} {Clause0_Item : Type} {Clause0_IntoIter : Type}
   {Clause2_IntoIter : Type} (coreitertraitscollectIntoIteratorInst :
   core.iter.traits.collect.IntoIterator I Clause0_Item Clause0_IntoIter)
   (coreborrowBorrowClause0_ItemScalarInst : core.borrow.Borrow Clause0_Item
   scalar.Scalar)
-  (coreitertraitscollectIntoIteratorJOptionRistrettoPointClause2_IntoIterInst :
-  core.iter.traits.collect.IntoIterator J (Option ristretto.RistrettoPoint)
-  Clause2_IntoIter) :
-  I → J → Result (Option ristretto.RistrettoPoint)
+  («coreitertraitscollectIntoIteratorJOptionRistrettoPointx86_64-unknown-linux-gnuClause2_IntoIterInst»
+  : core.iter.traits.collect.IntoIterator J (Option
+  ristretto.RistrettoPoint.«x86_64-unknown-linux-gnu») Clause2_IntoIter) :
+  I → J → Result (Option
+    ristretto.RistrettoPoint.«x86_64-unknown-linux-gnu»)
 
-/-- [curve25519_dalek::ristretto::{impl curve25519_dalek::traits::VartimePrecomputedMultiscalarMul<curve25519_dalek::ristretto::RistrettoPoint> for curve25519_dalek::ristretto::VartimeRistrettoPrecomputation}::optional_mixed_multiscalar_mul]:
+/-- [curve25519_dalek::ristretto::{impl curve25519_dalek::traits::VartimeMultiscalarMul<curve25519_dalek::ristretto::RistrettoPoint::i686-unknown-linux-gnu> for curve25519_dalek::ristretto::RistrettoPoint::i686-unknown-linux-gnu}::optional_multiscalar_mul]:
+    Source: 'curve25519-dalek/src/ristretto.rs', lines 1000:4-1012:5
+    Visibility: public -/
+axiom
+  ristretto.RistrettoPoint.«i686-unknown-linux-gnu».Insts.«Curve25519_dalekTraitsVartimeMultiscalarMulRistrettoPointi686-unknown-linux-gnu».optional_multiscalar_mul
+  {I : Type} {J : Type} {Clause0_Item : Type} {Clause0_IntoIter : Type}
+  {Clause2_IntoIter : Type} (coreitertraitscollectIntoIteratorInst :
+  core.iter.traits.collect.IntoIterator I Clause0_Item Clause0_IntoIter)
+  (coreborrowBorrowClause0_ItemScalarInst : core.borrow.Borrow Clause0_Item
+  scalar.Scalar)
+  («coreitertraitscollectIntoIteratorJOptionRistrettoPointi686-unknown-linux-gnuClause2_IntoIterInst»
+  : core.iter.traits.collect.IntoIterator J (Option
+  ristretto.RistrettoPoint.«i686-unknown-linux-gnu») Clause2_IntoIter) :
+  I → J → Result (Option
+    ristretto.RistrettoPoint.«i686-unknown-linux-gnu»)
+
+/-- [curve25519_dalek::ristretto::{impl curve25519_dalek::traits::VartimePrecomputedMultiscalarMul<curve25519_dalek::ristretto::RistrettoPoint::x86_64-unknown-linux-gnu> for curve25519_dalek::ristretto::VartimeRistrettoPrecomputation::x86_64-unknown-linux-gnu}::optional_mixed_multiscalar_mul]:
     Source: 'curve25519-dalek/src/ristretto.rs', lines 1047:4-1070:5
     Visibility: public -/
 axiom
-  ristretto.VartimeRistrettoPrecomputation.Insts.Curve25519_dalekTraitsVartimePrecomputedMultiscalarMulRistrettoPoint.optional_mixed_multiscalar_mul
+  ristretto.VartimeRistrettoPrecomputation.«x86_64-unknown-linux-gnu».Insts.«Curve25519_dalekTraitsVartimePrecomputedMultiscalarMulRistrettoPointx86_64-unknown-linux-gnu».optional_mixed_multiscalar_mul
   {I : Type} {J : Type} {K : Type} {Clause0_Item : Type} {Clause0_IntoIter :
   Type} {Clause2_Item : Type} {Clause2_IntoIter : Type} {Clause4_IntoIter :
   Type} (coreitertraitscollectIntoIteratorInst :
@@ -488,23 +721,61 @@ axiom
   core.iter.traits.collect.IntoIterator J Clause2_Item Clause2_IntoIter)
   (coreborrowBorrowClause2_ItemScalarInst : core.borrow.Borrow Clause2_Item
   scalar.Scalar)
-  (coreitertraitscollectIntoIteratorKOptionRistrettoPointClause4_IntoIterInst :
-  core.iter.traits.collect.IntoIterator K (Option ristretto.RistrettoPoint)
-  Clause4_IntoIter) :
-  ristretto.VartimeRistrettoPrecomputation → I → J → K → Result (Option
-    ristretto.RistrettoPoint)
+  («coreitertraitscollectIntoIteratorKOptionRistrettoPointx86_64-unknown-linux-gnuClause4_IntoIterInst»
+  : core.iter.traits.collect.IntoIterator K (Option
+  ristretto.RistrettoPoint.«x86_64-unknown-linux-gnu») Clause4_IntoIter) :
+  ristretto.VartimeRistrettoPrecomputation.«x86_64-unknown-linux-gnu» → I
+    → J → K → Result (Option
+    ristretto.RistrettoPoint.«x86_64-unknown-linux-gnu»)
 
-/-- [curve25519_dalek::ristretto::{impl curve25519_dalek::traits::VartimePrecomputedMultiscalarMul<curve25519_dalek::ristretto::RistrettoPoint> for curve25519_dalek::ristretto::VartimeRistrettoPrecomputation}::new]:
+/-- [curve25519_dalek::ristretto::{impl curve25519_dalek::traits::VartimePrecomputedMultiscalarMul<curve25519_dalek::ristretto::RistrettoPoint::x86_64-unknown-linux-gnu> for curve25519_dalek::ristretto::VartimeRistrettoPrecomputation::x86_64-unknown-linux-gnu}::new]:
     Source: 'curve25519-dalek/src/ristretto.rs', lines 1029:4-1037:5
     Visibility: public -/
 axiom
-  ristretto.VartimeRistrettoPrecomputation.Insts.Curve25519_dalekTraitsVartimePrecomputedMultiscalarMulRistrettoPoint.new
+  ristretto.VartimeRistrettoPrecomputation.«x86_64-unknown-linux-gnu».Insts.«Curve25519_dalekTraitsVartimePrecomputedMultiscalarMulRistrettoPointx86_64-unknown-linux-gnu».new
   {I : Type} {Clause0_Item : Type} {Clause0_IntoIter : Type}
   (coreitertraitscollectIntoIteratorInst :
   core.iter.traits.collect.IntoIterator I Clause0_Item Clause0_IntoIter)
-  (coreborrowBorrowClause0_ItemRistrettoPointInst : core.borrow.Borrow
-  Clause0_Item ristretto.RistrettoPoint) :
-  I → Result ristretto.VartimeRistrettoPrecomputation
+  («coreborrowBorrowClause0_ItemRistrettoPointx86_64-unknown-linux-gnuInst» :
+  core.borrow.Borrow Clause0_Item
+  ristretto.RistrettoPoint.«x86_64-unknown-linux-gnu») :
+  I → Result
+    ristretto.VartimeRistrettoPrecomputation.«x86_64-unknown-linux-gnu»
+
+/-- [curve25519_dalek::ristretto::{impl curve25519_dalek::traits::VartimePrecomputedMultiscalarMul<curve25519_dalek::ristretto::RistrettoPoint::i686-unknown-linux-gnu> for curve25519_dalek::ristretto::VartimeRistrettoPrecomputation::i686-unknown-linux-gnu}::optional_mixed_multiscalar_mul]:
+    Source: 'curve25519-dalek/src/ristretto.rs', lines 1047:4-1070:5
+    Visibility: public -/
+axiom
+  ristretto.VartimeRistrettoPrecomputation.«i686-unknown-linux-gnu».Insts.«Curve25519_dalekTraitsVartimePrecomputedMultiscalarMulRistrettoPointi686-unknown-linux-gnu».optional_mixed_multiscalar_mul
+  {I : Type} {J : Type} {K : Type} {Clause0_Item : Type} {Clause0_IntoIter :
+  Type} {Clause2_Item : Type} {Clause2_IntoIter : Type} {Clause4_IntoIter :
+  Type} (coreitertraitscollectIntoIteratorInst :
+  core.iter.traits.collect.IntoIterator I Clause0_Item Clause0_IntoIter)
+  (coreborrowBorrowClause0_ItemScalarInst : core.borrow.Borrow Clause0_Item
+  scalar.Scalar) (coreitertraitscollectIntoIteratorInst1 :
+  core.iter.traits.collect.IntoIterator J Clause2_Item Clause2_IntoIter)
+  (coreborrowBorrowClause2_ItemScalarInst : core.borrow.Borrow Clause2_Item
+  scalar.Scalar)
+  («coreitertraitscollectIntoIteratorKOptionRistrettoPointi686-unknown-linux-gnuClause4_IntoIterInst»
+  : core.iter.traits.collect.IntoIterator K (Option
+  ristretto.RistrettoPoint.«i686-unknown-linux-gnu») Clause4_IntoIter) :
+  ristretto.VartimeRistrettoPrecomputation.«i686-unknown-linux-gnu» → I →
+    J → K → Result (Option
+    ristretto.RistrettoPoint.«i686-unknown-linux-gnu»)
+
+/-- [curve25519_dalek::ristretto::{impl curve25519_dalek::traits::VartimePrecomputedMultiscalarMul<curve25519_dalek::ristretto::RistrettoPoint::i686-unknown-linux-gnu> for curve25519_dalek::ristretto::VartimeRistrettoPrecomputation::i686-unknown-linux-gnu}::new]:
+    Source: 'curve25519-dalek/src/ristretto.rs', lines 1029:4-1037:5
+    Visibility: public -/
+axiom
+  ristretto.VartimeRistrettoPrecomputation.«i686-unknown-linux-gnu».Insts.«Curve25519_dalekTraitsVartimePrecomputedMultiscalarMulRistrettoPointi686-unknown-linux-gnu».new
+  {I : Type} {Clause0_Item : Type} {Clause0_IntoIter : Type}
+  (coreitertraitscollectIntoIteratorInst :
+  core.iter.traits.collect.IntoIterator I Clause0_Item Clause0_IntoIter)
+  («coreborrowBorrowClause0_ItemRistrettoPointi686-unknown-linux-gnuInst» :
+  core.borrow.Borrow Clause0_Item
+  ristretto.RistrettoPoint.«i686-unknown-linux-gnu») :
+  I → Result
+    ristretto.VartimeRistrettoPrecomputation.«i686-unknown-linux-gnu»
 
 /-- [curve25519_dalek::scalar::{impl core::iter::traits::accum::Product<T> for curve25519_dalek::scalar::Scalar}::product]:
     Source: 'curve25519-dalek/src/scalar.rs', lines 458:4-463:5
